Tweak handling of virtual addresses for indirect sentry invocations
Require specific address for code caps in load pair instructions, even
in the case of not invoking a direct sentry, but where the loaded cap
happens to be a direct sentry.

Moreover, in the invocation case split lemma, be more explicit about the
physical addresses.  The set of accessed physical addresses will always
have at most one or two elements, whereas for virtual addresses, that
would be tricky to state with potentially non-injective address
mappings.

CHERI_Instantiation.thy
@@ -1896,13 +1896,15 @@ definition trace_is_in_c64 :: "register_value trace \<Rightarrow> bool" where
 definition trace_load_auths :: "register_value trace \<Rightarrow> load_auth option" where
   "trace_load_auths t \<equiv> Option.bind (instr_of_trace t) instr_load_auth"
 
-definition trace_has_cap_load_auth :: "register_value trace \<Rightarrow> bool" where
-  "trace_has_cap_load_auth t \<equiv>
-     (\<exists>auth r c.
+definition load_auth_caps_of_trace :: "register_value trace \<Rightarrow> Capability set" where
+  "load_auth_caps_of_trace t \<equiv>
+     {c. \<exists>r auth.
         trace_load_auths t = Some auth \<and>
         r \<in> load_auth_reg_names (trace_is_in_c64 t) auth \<and>
-        E_read_reg r (Regval_bitvector_129_dec c) \<in> set t \<and>
-        cap_permits CAP_PERM_LOAD_CAP c)"
+        E_read_reg r (Regval_bitvector_129_dec c) \<in> set t}"
+
+definition trace_has_cap_load_auth :: "register_value trace \<Rightarrow> bool" where
+  "trace_has_cap_load_auth t \<equiv> (\<exists>c \<in> load_auth_caps_of_trace t. cap_permits CAP_PERM_LOAD_CAP c)"
 
 definition trace_uses_mem_caps :: "(register_value, instr) isa_trace \<Rightarrow> bool" where
   "trace_uses_mem_caps t \<equiv> trace_has_cap_load_auth (trace t)"
@@ -2084,6 +2086,9 @@ definition original_direct_mem_sentries_invoked_in_trace :: "register_value trac
          trace_invokes_indirect_sentries t = {} \<and>
          trace_has_cap_load_auth t \<and>
          reads_mem_cap CC e = Some (addr, nat CAPABILITY_DBYTES, c) \<and>
+         (trace_indirect_sentry_type t = Some Points_to_Pair \<longrightarrow>
+            (\<exists>auth \<in> load_auth_caps_of_trace t.
+               translate_address (unat (CapGetValue auth + 16)) = Some addr)) \<and>
          CapIsTagSet c \<and> is_sentry c}"
 
 definition trace_invokes_direct_mem_sentries :: "register_value trace \<Rightarrow> Capability set" where
@@ -6205,11 +6210,11 @@ locale Morello_Cap_Invocation_Assms = Morello_ISA +
   fixes enabled :: "(Capability, register_value) axiom_state \<Rightarrow> register_value event \<Rightarrow> bool"
     and use_mem_caps :: "bool"
     and instr_opt :: "instr_ast option"
-    (* TODO: Just fix `instr` instead of regs and sentry_type? *)
     and invoked_code_caps :: "Capability set"
     and invoked_data_caps :: "Capability set"
     and invoked_indirect_caps :: "Capability set"
     and original_reg_code_caps :: "Capability set"
+    and original_reg_load_auth_caps :: "Capability set"
 begin
 
 abbreviation "invoked_code_reg \<equiv> Option.bind instr_opt instr_invokes_code_cap_from_reg"
@@ -6225,9 +6230,10 @@ fun invocation_ev_assms :: "register_value event \<Rightarrow> bool" where
      (\<forall>n cc cd. r \<in> R_name n \<and> invoked_data_reg = Some n \<and> cd \<in> caps_of_regval v \<and> cc \<in> original_reg_code_caps \<and> invokable CC cc cd
         \<longrightarrow> CapUnseal cd \<in> invoked_data_caps \<and> branch_caps (clear_lsb (CapUnseal cc)) \<subseteq> invoked_code_caps) \<and>
      (\<forall>n c sentry_type. r \<in> R_name n \<and> invoked_indirect_reg = Some n \<and> c \<in> caps_of_regval v \<and> indirect_sentry_type = Some sentry_type
-         \<longrightarrow> (if CapIsTagSet c \<and> CapIsSealed c \<and> get_indirect_sentry_type c = Some sentry_type
+         \<longrightarrow> (if CapIsTagSet c \<and> CapIsSealed c \<and> get_indirect_sentry_type c = Some sentry_type \<comment> \<open>\<and> cap_permits CAP_PERM_LOAD_CAP c\<close>
               then invoked_indirect_caps = {CapUnseal c} \<and> (sentry_type = Points_to_PCC \<longrightarrow> CapUnseal c \<in> invoked_data_caps) \<comment> \<open>Points-to-PCC sentry becomes data cap\<close>
-              else invoked_indirect_caps = {})))"
+              else invoked_indirect_caps = {})) \<and>
+     (\<forall>n c. Option.bind instr_opt instr_load_auth = Some (RegAuth n) \<and> r \<in> R_name n \<and> c \<in> caps_of_regval v \<longrightarrow> c \<in> original_reg_load_auth_caps))"
 | "invocation_ev_assms (E_read_memt rk paddr sz (bytes, tag)) \<longleftrightarrow>
     (case indirect_sentry_type of
        Some sentry_type \<Rightarrow>
@@ -6247,7 +6253,10 @@ fun invocation_ev_assms :: "register_value event \<Rightarrow> bool" where
              | Points_to_PCC \<Rightarrow> mem_branch_caps (clear_lsb c) \<subseteq> invoked_code_caps))
      | None \<Rightarrow> True) \<and>
     (is_indirect_branch \<and> invoked_indirect_caps = {} \<and> use_mem_caps \<longrightarrow>
-       (\<forall>c. cap_of_mem_bytes bytes tag = Some c \<and> sz = nat CAPABILITY_DBYTES \<and> CapIsTagSet c \<and> is_sentry c \<longrightarrow>
+       (\<forall>c. cap_of_mem_bytes bytes tag = Some c \<and> sz = nat CAPABILITY_DBYTES \<and> CapIsTagSet c \<and> is_sentry c \<and>
+              (indirect_sentry_type = Some Points_to_Pair \<longrightarrow>
+                 (\<exists>auth \<in> original_reg_load_auth_caps. translate_address (unat (CapGetValue auth + 16)) = Some paddr))
+            \<longrightarrow>
             mem_branch_caps (clear_lsb c) \<subseteq> invoked_code_caps))"
 | "invocation_ev_assms _ = True"
 
@@ -6338,6 +6347,7 @@ lemma instantiated_invocation_trace_assms:
     and "invoked_data_caps = instr_invokes_data_caps opcode t"
     and "invoked_indirect_caps = trace_invokes_indirect_sentries t"
     and "original_reg_code_caps = original_reg_code_caps_read_in_trace t"
+    and "original_reg_load_auth_caps = load_auth_caps_of_trace t"
     and "use_mem_caps \<longrightarrow> trace_has_cap_load_auth t"
   shows "invocation_trace_assms t"
 proof (unfold invocation_trace_assms_def, intro ballI)
@@ -6367,21 +6377,21 @@ proof (unfold invocation_trace_assms_def, intro ballI)
         unfolding invocation_ev_assms.simps
         apply (cases rule: instr_of_trace_invocation_cases[OF Some', where opcode = opcode])
         subgoal
-          by (auto simp: original_reg_code_caps_read_in_trace_def trace_invokes_code_cap_from_reg_def trace_reads_caps_from_gpr_def instr_invokes_indirect_caps_def no_code_or_data_cap_regs_if_indirect_cap_regs)
+          by (auto simp: original_reg_code_caps_read_in_trace_def trace_invokes_code_cap_from_reg_def trace_reads_caps_from_gpr_def instr_invokes_indirect_caps_def no_code_or_data_cap_regs_if_indirect_cap_regs load_auth_caps_of_trace_def trace_load_auths_def)
         subgoal
-          by (auto simp: original_reg_code_caps_read_in_trace_def trace_invokes_code_cap_from_reg_def trace_reads_caps_from_gpr_def instr_invokes_indirect_caps_def no_code_or_data_cap_regs_if_indirect_cap_regs)
+          by (auto simp: original_reg_code_caps_read_in_trace_def trace_invokes_code_cap_from_reg_def trace_reads_caps_from_gpr_def instr_invokes_indirect_caps_def no_code_or_data_cap_regs_if_indirect_cap_regs load_auth_caps_of_trace_def trace_load_auths_def)
         subgoal
-          by (auto simp: original_reg_code_caps_read_in_trace_def trace_invokes_code_cap_from_reg_def trace_reads_caps_from_gpr_def instr_invokes_indirect_caps_def no_code_or_data_cap_regs_if_indirect_cap_regs)
+          by (auto simp: original_reg_code_caps_read_in_trace_def trace_invokes_code_cap_from_reg_def trace_reads_caps_from_gpr_def instr_invokes_indirect_caps_def no_code_or_data_cap_regs_if_indirect_cap_regs load_auth_caps_of_trace_def trace_load_auths_def)
         subgoal
-          apply (auto simp: original_reg_code_caps_read_in_trace_def trace_invokes_code_cap_from_reg_def trace_reads_caps_from_gpr_def instr_invokes_indirect_caps_def no_code_or_data_cap_regs_if_indirect_cap_regs CapIsSealed_def)
+          apply (auto simp: original_reg_code_caps_read_in_trace_def trace_invokes_code_cap_from_reg_def trace_reads_caps_from_gpr_def instr_invokes_indirect_caps_def no_code_or_data_cap_regs_if_indirect_cap_regs CapIsSealed_def load_auth_caps_of_trace_def trace_load_auths_def)
           (* TODO: Uniqueness of cap in invoked indirect register *)
           sorry
         subgoal
-          apply (auto simp: original_reg_code_caps_read_in_trace_def trace_invokes_code_cap_from_reg_def trace_reads_caps_from_gpr_def instr_invokes_indirect_caps_def no_code_or_data_cap_regs_if_indirect_cap_regs CapIsSealed_def)
+          apply (auto simp: original_reg_code_caps_read_in_trace_def trace_invokes_code_cap_from_reg_def trace_reads_caps_from_gpr_def instr_invokes_indirect_caps_def no_code_or_data_cap_regs_if_indirect_cap_regs CapIsSealed_def load_auth_caps_of_trace_def trace_load_auths_def)
           (* TODO: Uniqueness of cap in invoked indirect register *)
           sorry
         subgoal
-          apply (auto simp: instr_invokes_code_caps_def instr_invokes_data_caps_def instr_invokes_indirect_caps_def original_reg_code_caps_read_in_trace_def trace_reads_caps_from_gpr_def)
+          apply (auto simp: instr_invokes_code_caps_def instr_invokes_data_caps_def instr_invokes_indirect_caps_def original_reg_code_caps_read_in_trace_def trace_reads_caps_from_gpr_def load_auth_caps_of_trace_def trace_load_auths_def)
           subgoal
             by (auto simp: trace_invokes_reg_code_caps_def original_reg_code_caps_invoked_in_trace_def original_direct_reg_sentries_invoked_in_trace_def trace_reads_caps_from_gpr_def simp flip: clear_lsb_image_branch_caps_eq)
           subgoal
@@ -6408,11 +6418,12 @@ proof (unfold invocation_trace_assms_def, intro ballI)
         subgoal by (auto simp: no_code_or_data_cap_regs_if_indirect_sentry split: option.split)
         subgoal by (auto simp: no_code_or_data_cap_regs_if_indirect_sentry split: option.split)
         subgoal
-          apply (auto simp: instr_invokes_indirect_caps_def mem_branch_caps_def CapUnseal_clear_lsb_commute is_sentry_def CapIsSealed_def reads_mem_cap_Some_iff')
+          apply (auto simp: instr_invokes_indirect_caps_def mem_branch_caps_def CapUnseal_clear_lsb_commute is_sentry_def CapIsSealed_def reads_mem_cap_Some_iff' load_auth_caps_of_trace_def trace_load_auths_def)
+          apply fastforce
           apply fastforce
           done
         subgoal
-          apply (auto simp: instr_invokes_indirect_caps_def instr_invokes_code_caps_def is_sentry_def CapIsSealed_def reads_mem_cap_Some_iff')
+          apply (auto simp: instr_invokes_indirect_caps_def instr_invokes_code_caps_def is_sentry_def CapIsSealed_def reads_mem_cap_Some_iff' load_auth_caps_of_trace_def trace_load_auths_def)
            apply fastforce
           done
         subgoal
@@ -6422,6 +6433,7 @@ proof (unfold invocation_trace_assms_def, intro ballI)
           done
         subgoal
           apply (auto simp: instr_invokes_indirect_caps_def instr_invokes_code_caps_def trace_invokes_direct_mem_sentries_def original_direct_mem_sentries_invoked_in_trace_def reads_mem_cap_Some_iff' image_UN clear_lsb_image_mem_branch_caps_eq split: option.split)
+          apply fastforce
           apply fastforce
           done
         done
@@ -6526,6 +6538,19 @@ proof -
     by (auto simp: is_sentry_def)
 qed
 
+lemma C_read_original_reg_load_auth_caps[derivable_capsE]:
+  assumes "Run (C_read n) t c" and "invocation_trace_assms t"
+    and "Option.bind instr_opt instr_load_auth = Some (RegAuth n)"
+    and "CapIsTagSet c"
+  shows "c \<in> original_reg_load_auth_caps"
+proof -
+  obtain r where "invocation_ev_assms (E_read_reg r (Regval_bitvector_129_dec c))" and "r \<in> R_name n"
+    using assms(1,2,4)
+    by (elim Run_C_readE) (auto simp: CapNull_def invocation_trace_assms_def)
+  with assms(3-) show ?thesis
+    by auto
+qed
+
 lemma CapGetObjectType_get_indirect_sentry_type[unfolded special_otype_defs, simp]:
   "CapGetObjectType c = CAP_SEAL_TYPE_LB \<Longrightarrow> get_indirect_sentry_type c = Some Points_to_PCC"
   "CapGetObjectType c = CAP_SEAL_TYPE_LPB \<Longrightarrow> get_indirect_sentry_type c = Some Points_to_Pair"
@@ -6580,6 +6605,26 @@ lemma CSP_or_C_read_unseal_invoked_indirect_caps:
   shows "CapUnseal c \<in> invoked_indirect_caps"
   using assms
   by (auto elim!: C_read_unseal_invoked_indirect_caps_cases CSP_read_invoked_indirect_caps_cases Run_bindE split: if_splits)
+
+lemma CSP_read_original_reg_load_auth_caps[derivable_capsE]:
+  assumes "Run (CSP_read u) t c" and "invocation_trace_assms t"
+    and "Option.bind instr_opt instr_load_auth = Some (RegAuth 31)"
+  shows "c \<in> original_reg_load_auth_caps"
+proof -
+  obtain r where "invocation_ev_assms (E_read_reg r (Regval_bitvector_129_dec c))" and "r \<in> R_name 31"
+    using assms(1,2)
+    by (elim Run_CSP_readE) (auto simp: invocation_trace_assms_def)
+  with assms(3) show ?thesis
+    by auto
+qed
+
+lemma CSP_or_C_read_original_reg_load_auth_caps[derivable_capsE]:
+  assumes "Run (if n = 31 then CheckSPAlignment u \<then> CSP_read u' else C_read n) t c" and "invocation_trace_assms t"
+    and "Option.bind instr_opt instr_load_auth = Some (RegAuth n)"
+    and "CapIsTagSet c"
+  shows "c \<in> original_reg_load_auth_caps"
+  using assms
+  by (auto elim!: CSP_read_original_reg_load_auth_caps C_read_original_reg_load_auth_caps Run_bindE split: if_splits)
 
 declare Run_ifE[where thesis = "CapUnseal c \<in> invoked_indirect_caps" and a = c for c, derivable_caps_combinators]
 declare Run_bindE[where thesis = "CapUnseal c \<in> invoked_indirect_caps" and a = c for c, derivable_caps_combinators]
@@ -6811,14 +6856,16 @@ lemma mem_cap_vaddr_loaded_in_trace_if_tagged_invoked_direct_mem_sentry:
     and "CapIsTagSet c"
     and "is_sentry c"
     and "is_indirect_branch"
+    and "indirect_sentry_type = Some Points_to_Pair \<longrightarrow>
+           (\<exists>auth \<in> original_reg_load_auth_caps. vaddr = unat (CapGetValue auth + 16))"
     and "invoked_indirect_caps = {}"
     and "use_mem_caps"
   shows "mem_branch_caps (clear_lsb c) \<subseteq> invoked_code_caps"
-  using assms(1-5)
+  using assms(1-6)
   unfolding mem_cap_vaddr_loaded_in_trace_if_tagged_def mem_cap_vaddr_loads_of_trace_def
   apply (auto simp: invocation_trace_assms_def elim!: mem_cap_loads_of_traceE mem_cap_loads_of_evE
            dest!: invocation_trace_assmsD[OF assms(2)] split: if_splits)
-  apply (auto simp: assms(6,7))
+  apply (auto simp: assms(7,8))
   done
 
 (* *** Merge *** *)
@@ -6860,9 +6907,10 @@ locale Morello_Axiom_Assms = Morello_ISA +
     and invoked_data_caps :: "Capability set"
     and invoked_indirect_caps :: "Capability set"
     and original_reg_code_caps :: "Capability set"
+    and original_reg_load_auth_caps :: "Capability set"
     (*and invoked_caps :: "Capability set" and invoked_regs :: "int set"
     and invoked_indirect_caps :: "Capability set" and invoked_indirect_regs :: "int set"*)
-    and load_auth :: "load_auth option" and load_caps_permitted :: "bool"
+    and load_caps_permitted :: "bool"
     and no_system_reg_access :: bool
     and is_in_c64 :: bool
 
@@ -6874,7 +6922,9 @@ locale Morello_Axiom_Assms = Morello_ISA +
     (* and translation_assms :: "register_value event \<Rightarrow> bool" *)
 begin
 
-sublocale Morello_Load_Cap_Assms ..
+abbreviation "load_auth \<equiv> Option.bind instr_opt instr_load_auth"
+
+sublocale Morello_Load_Cap_Assms where load_auth = load_auth ..
 sublocale Morello_Cap_Invocation_Assms
  (* where use_mem_caps = "invoked_indirect_caps = {} \<and> load_caps_permitted" .. *)
   where use_mem_caps = load_caps_permitted ..
@@ -7149,7 +7199,8 @@ locale Morello_Write_Cap_Automaton = Morello_ISA +
     and invoked_data_caps :: "Capability set"
     and invoked_indirect_caps :: "Capability set"
     and original_reg_code_caps :: "Capability set"
-    and load_auth :: "load_auth option" and load_caps_permitted :: "bool"
+    and original_reg_load_auth_caps :: "Capability set"
+    and load_caps_permitted :: "bool"
     and no_system_reg_access :: bool
     and is_in_c64 :: bool
     and is_fetch :: "bool"
@@ -7194,7 +7245,8 @@ locale Morello_Mem_Axiom_Automaton = Morello_ISA +
     and invoked_data_caps :: "Capability set"
     and invoked_indirect_caps :: "Capability set"
     and original_reg_code_caps :: "Capability set"
-    and load_auth :: "load_auth option" and load_caps_permitted :: "bool"
+    and original_reg_load_auth_caps :: "Capability set"
+    and load_caps_permitted :: "bool"
     and no_system_reg_access :: bool
     and is_in_c64 :: bool
     and is_fetch :: "bool"
@@ -7260,7 +7312,7 @@ locale Morello_Trace_Axiom_Automaton = Morello_ISA +
     and invoked_data_caps = "trace_invokes_data_caps ISA t"
     and invoked_indirect_caps = "trace_invokes_indirect_caps ISA t"
     and original_reg_code_caps = "original_reg_code_caps_read_in_trace (trace t)"
-    and load_auth = "trace_load_auths (trace t)"
+    and original_reg_load_auth_caps = "load_auth_caps_of_trace (trace t)"
     and load_caps_permitted = "isa.trace_uses_mem_caps ISA t"
     and no_system_reg_access = "\<not>trace_has_system_reg_access (trace t)"
     and is_in_c64 = "trace_is_in_c64 (trace t)"
@@ -7275,7 +7327,7 @@ locale Morello_Trace_Write_Cap_Automaton = Morello_ISA +
     and invoked_data_caps = "trace_invokes_data_caps ISA t"
     and invoked_indirect_caps = "trace_invokes_indirect_caps ISA t"
     and original_reg_code_caps = "original_reg_code_caps_read_in_trace (trace t)"
-    and load_auth = "trace_load_auths (trace t)"
+    and original_reg_load_auth_caps = "load_auth_caps_of_trace (trace t)"
     and load_caps_permitted = "isa.trace_uses_mem_caps ISA t"
     and no_system_reg_access = "\<not>trace_has_system_reg_access (trace t)"
     and is_in_c64 = "trace_is_in_c64 (trace t)"
@@ -7292,7 +7344,7 @@ locale Morello_Trace_Mem_Automaton = Morello_ISA +
     and invoked_data_caps = "trace_invokes_data_caps ISA t"
     and invoked_indirect_caps = "trace_invokes_indirect_caps ISA t"
     and original_reg_code_caps = "original_reg_code_caps_read_in_trace (trace t)"
-    and load_auth = "trace_load_auths (trace t)"
+    and original_reg_load_auth_caps = "load_auth_caps_of_trace (trace t)"
     and load_caps_permitted = "isa.trace_uses_mem_caps ISA t"
     and no_system_reg_access = "\<not>trace_has_system_reg_access (trace t)"
     and is_in_c64 = "trace_is_in_c64 (trace t)"
@@ -7312,7 +7364,7 @@ sublocale Morello_Instr_Trace_Axiom_Automaton \<subseteq> Morello_Instr_Axiom_Au
     and invoked_data_caps = "trace_invokes_data_caps ISA (instr_trace instr t)"
     and invoked_indirect_caps = "trace_invokes_indirect_caps ISA (instr_trace instr t)"
     and original_reg_code_caps = "original_reg_code_caps_read_in_trace (trace (instr_trace instr t))"
-    and load_auth = "trace_load_auths (trace (instr_trace instr t))"
+    and original_reg_load_auth_caps = "load_auth_caps_of_trace (trace (instr_trace instr t))"
     and load_caps_permitted = "isa.trace_uses_mem_caps ISA (instr_trace instr t)"
     and no_system_reg_access = "\<not>trace_has_system_reg_access (trace (instr_trace instr t))"
     and is_in_c64 = "trace_is_in_c64 (trace (instr_trace instr t))"
@@ -7330,7 +7382,7 @@ sublocale Morello_Fetch_Trace_Axiom_Automaton \<subseteq> Morello_Fetch_Axiom_Au
     and invoked_data_caps = "trace_invokes_data_caps ISA (fetch_trace t :: (register_value, instr) isa_trace)"
     and invoked_indirect_caps = "trace_invokes_indirect_caps ISA (fetch_trace t :: (register_value, instr) isa_trace)"
     and original_reg_code_caps = "original_reg_code_caps_read_in_trace (trace (fetch_trace t :: (register_value, instr) isa_trace))"
-    and load_auth = "trace_load_auths (trace (fetch_trace t :: (register_value, instr) isa_trace))"
+    and original_reg_load_auth_caps = "load_auth_caps_of_trace (trace (fetch_trace t :: (register_value, instr) isa_trace))"
     and load_caps_permitted = "isa.trace_uses_mem_caps ISA (fetch_trace t :: (register_value, instr) isa_trace)"
     and no_system_reg_access = "\<not>trace_has_system_reg_access (trace (fetch_trace t :: (register_value, instr) isa_trace))"
     and is_in_c64 = "trace_is_in_c64 (trace (fetch_trace t :: (register_value, instr) isa_trace))"
@@ -7351,7 +7403,7 @@ sublocale Morello_Instr_Trace_Write_Cap_Automaton \<subseteq> Morello_Instr_Writ
     and invoked_data_caps = "trace_invokes_data_caps ISA (instr_trace instr t)"
     and invoked_indirect_caps = "trace_invokes_indirect_caps ISA (instr_trace instr t)"
     and original_reg_code_caps = "original_reg_code_caps_read_in_trace (trace (instr_trace instr t))"
-    and load_auth = "trace_load_auths (trace (instr_trace instr t))"
+    and original_reg_load_auth_caps = "load_auth_caps_of_trace (trace (instr_trace instr t))"
     and load_caps_permitted = "isa.trace_uses_mem_caps ISA (instr_trace instr t)"
     and no_system_reg_access = "\<not>trace_has_system_reg_access (trace (instr_trace instr t))"
     and is_in_c64 = "trace_is_in_c64 (trace (instr_trace instr t))"
@@ -7372,7 +7424,7 @@ sublocale Morello_Instr_Trace_Mem_Automaton \<subseteq> Morello_Instr_Mem_Automa
     and invoked_data_caps = "trace_invokes_data_caps ISA (instr_trace instr t)"
     and invoked_indirect_caps = "trace_invokes_indirect_caps ISA (instr_trace instr t)"
     and original_reg_code_caps = "original_reg_code_caps_read_in_trace (trace (instr_trace instr t))"
-    and load_auth = "trace_load_auths (trace (instr_trace instr t))"
+    and original_reg_load_auth_caps = "load_auth_caps_of_trace (trace (instr_trace instr t))"
     and load_caps_permitted = "isa.trace_uses_mem_caps ISA (instr_trace instr t)"
     and no_system_reg_access = "\<not>trace_has_system_reg_access (trace (instr_trace instr t))"
     and is_in_c64 = "trace_is_in_c64 (trace (instr_trace instr t))"
@@ -7393,7 +7445,7 @@ sublocale Morello_Fetch_Trace_Write_Cap_Automaton \<subseteq> Morello_Fetch_Writ
     and invoked_data_caps = "trace_invokes_data_caps ISA (fetch_trace t :: (register_value, instr) isa_trace)"
     and invoked_indirect_caps = "trace_invokes_indirect_caps ISA (fetch_trace t :: (register_value, instr) isa_trace)"
     and original_reg_code_caps = "original_reg_code_caps_read_in_trace (trace (fetch_trace t :: (register_value, instr) isa_trace))"
-    and load_auth = "trace_load_auths (trace (fetch_trace t :: (register_value, instr) isa_trace))"
+    and original_reg_load_auth_caps = "load_auth_caps_of_trace (trace (fetch_trace t :: (register_value, instr) isa_trace))"
     and load_caps_permitted = "isa.trace_uses_mem_caps ISA (fetch_trace t :: (register_value, instr) isa_trace)"
     and no_system_reg_access = "\<not>trace_has_system_reg_access (trace (fetch_trace t :: (register_value, instr) isa_trace))"
     and is_in_c64 = "trace_is_in_c64 (trace (fetch_trace t :: (register_value, instr) isa_trace))"
@@ -7414,7 +7466,7 @@ sublocale Morello_Fetch_Trace_Mem_Automaton \<subseteq> Morello_Fetch_Mem_Automa
     and invoked_data_caps = "trace_invokes_data_caps ISA (fetch_trace t :: (register_value, instr) isa_trace)"
     and invoked_indirect_caps = "trace_invokes_indirect_caps ISA (fetch_trace t :: (register_value, instr) isa_trace)"
     and original_reg_code_caps = "original_reg_code_caps_read_in_trace (trace (fetch_trace t :: (register_value, instr) isa_trace))"
-    and load_auth = "trace_load_auths (trace (fetch_trace t :: (register_value, instr) isa_trace))"
+    and original_reg_load_auth_caps = "load_auth_caps_of_trace (trace (fetch_trace t :: (register_value, instr) isa_trace))"
     and load_caps_permitted = "isa.trace_uses_mem_caps ISA (fetch_trace t :: (register_value, instr) isa_trace)"
     and no_system_reg_access = "\<not>trace_has_system_reg_access (trace (fetch_trace t :: (register_value, instr) isa_trace))"
     and is_in_c64 = "trace_is_in_c64 (trace (fetch_trace t :: (register_value, instr) isa_trace))"
